DeBruijnSSA/BinSyntax/Rewrite.lean
@@ -1,1 +1,3 @@
 import DeBruijnSSA.BinSyntax.Rewrite.Definitions
+import DeBruijnSSA.BinSyntax.Rewrite.Subst
+import DeBruijnSSA.BinSyntax.Rewrite.Categorical
